cfrontend/BeePL_typechecker.v
@@ -1,0 +1,14 @@
+Require Import String ZArith Coq.FSets.FMapAVL Coq.Structures.OrderedTypeEx Coq.Strings.BinaryString.
+Require Import Coq.FSets.FSetProperties Coq.FSets.FMapFacts FMaps FSetAVL Nat PeanoNat Coq.Lists.List.
+Require Import Coq.Arith.EqNat Coq.ZArith.Int Integers AST Maps Ctypes.
+Require Import BeePL_aux BeePL BeeTypes BeePL_mem.
+
+(***** Type checker for BeePL *****)
+
+Definition type_constant (c : constant) : type :=
+match c with 
+| ConsInt i => (Ptype Tint)
+| ConsUint i => (Ptype Tuint)
+| ConsBool b => (Ptype Tbool)
+| ConsUnit => (Ptype Tunit)
+end.
